formic_site_duct/formic.apis.duct.dfy
@@ -1,0 +1,14 @@
+import opened DuctImpl
+import opened DuctApi
+
+class Views {
+    static method Endpoints() returns (all: AllApiEndpoints)
+        ensures |all.endpoints| == 1
+    {
+        var catalog := new AllApiEndpoints();
+        var generator := new FormicLandingPage();
+        var ep := new ApiEndpoint("/", ReturnType.Content, generator);
+        catalog.Add(ep);
+        return catalog;
+    }
+}
